src/checker.v
@@ -1,0 +1,122 @@
+Require Import Ast.
+Require Import ch2o.prelude.stringmap.
+Require Import ch2o.prelude.base.
+Require Import Coq.Strings.String.
+Require Import Coq.Bool.Sumbool.
+Require Import common.
+
+Definition ty_ctx := stringmap ty.
+
+Section checker.
+Context (P: program).
+Context (Γ: ty_ctx).
+
+Class Viewpoint (A B: Type) := adapt_viewpoint: A -> B -> B.
+Notation "a ⊳ b" := (adapt_viewpoint a b) (at level 60, right associativity) : C_scope.
+
+Class Alias (A: Type) := alias: A -> A.
+Class Subtype (A: Type) := is_subtype: A -> A -> bool.
+
+Instance viewpoint_cap: Viewpoint cap cap := {
+  adapt_viewpoint a b := match a, b with
+  | cap_iso, cap_iso => cap_iso
+  | cap_iso, cap_ref => cap_iso
+
+  | cap_ref, cap_iso => cap_iso
+  | cap_ref, cap_ref => cap_ref
+
+  | _, cap_tag => cap_tag
+
+  | cap_tag, _ => cap_tag
+  end
+}.
+
+Instance viewpoint_cap_ty: Viewpoint cap ty := {
+  adapt_viewpoint a b := match b with
+  | ty_name n c => ty_name n (a ⊳ c)
+  end
+}.
+
+Instance alias_cap : Alias cap := {
+  alias a := match a with
+  | cap_iso => cap_tag
+  | cap_ref => cap_ref
+  | cap_tag => cap_tag
+  end
+}.
+
+Instance alias_ty : Alias ty := {
+  alias a := match a with
+  | ty_name n c => ty_name n (alias c)
+  end
+}.
+
+Instance subtype_cap : Subtype cap := {
+  is_subtype a b := match a, b with
+  | cap_iso, cap_iso => true
+  | _, cap_tag => true
+  | _, _ => false
+  end
+}.
+
+Instance subtype_ty : Subtype ty := {
+  is_subtype a b :=
+    match a, b with
+    | ty_name name_a cap_a, ty_name name_b cap_b =>
+        if string_dec name_a name_b
+        then is_subtype cap_a cap_b
+        else false
+    end
+}.
+
+Fixpoint ck_expr (e: expr) : option ty :=
+  match e with
+  | expr_local x => Γ !! x
+  | expr_field e f =>
+      baset <- ck_expr e;
+      match baset with
+      | ty_name name cap =>
+          cls <- lookup_class name P;
+          fty <- lookup_field f cls;
+          Some (cap ⊳ fty)
+      end
+
+  | expr_assign_local x e =>
+      lhs <- Γ !! x;
+      rhs <- ck_expr e;
+      if is_subtype (alias rhs) lhs
+      then Some lhs
+      else None
+
+  | expr_ctor name ctor_name es =>
+      cls <- lookup_class name P;
+      '(args, _) <- lookup_ctor ctor_name cls;
+      _ <- ck_args es (map snd args);
+
+      Some (ty_name name cap_ref)
+
+  | expr_call e0 m es =>
+      baset <- ck_expr e0;
+      match baset with
+      | ty_name name cap =>
+          cls <- lookup_class name P;
+          '(reccap, args, retty, _) <- lookup_method m cls;
+          _ <- ck_args es (map snd args);
+
+          Some retty
+      end
+
+  | _ => None
+  end
+with
+  ck_args (es: list_expr) (args: list ty) : option unit :=
+    match es, args with
+    | list_expr_nil, nil => Some ()
+    | list_expr_cons e es', arg :: args' =>
+        ety <- ck_expr e;
+        if is_subtype (alias ety) arg
+        then ck_args es' args'
+        else None
+    | _, _ => None
+    end.
+End checker.
